src/lowparse/LowParse.Low.Int.fsti
@@ -13,15 +13,15 @@ val parse32_u32: parser32 parse_u32
 
 inline_for_extraction
 let validate32_u8 : validator32 parse_u8 =
-  validate32_total_constant_size parse_u8 1ul ()
+  validate32_total_constant_size parse_u8 1l ()
 
 inline_for_extraction
 let validate32_u16 : validator32 parse_u16 =
-  validate32_total_constant_size parse_u16 2ul ()
+  validate32_total_constant_size parse_u16 2l ()
 
 inline_for_extraction
 let validate32_u32 : validator32 parse_u32 =
-  validate32_total_constant_size parse_u32 4ul ()
+  validate32_total_constant_size parse_u32 4l ()
 
 inline_for_extraction
 let validate_nochk32_u8 : validator_nochk32 parse_u8 =
