src/lowparse/LowParseExample3.fst
@@ -6,22 +6,22 @@ module HST = FStar.HyperStack.ST
 module U32 = FStar.UInt32
 module U16 = FStar.UInt16
 module Cast = FStar.Int.Cast
+module I32 = FStar.Int32
 
 #reset-options "--z3rlimit 32"
 
 let dummy
   (input: buffer8)
-  (len: U32.t)
+  (len: I32.t)
   (which: U32.t)
 : HST.Stack U32.t
   (requires (fun h -> is_slice h input len))
   (ensures (fun _ _ _ -> True))
 = HST.push_frame ();
-  let input' = B.create input 1ul in
-  let len' = B.create len 1ul in
   let res =
-    if validate32_t input' len'
-    then
+    if validate32_t input len `I32.lt` 0l
+    then 0ul
+    else
       if which = 42ul
       then
         let x : U16.t = read_from_buffer access_a parse32_u16 input in
@@ -32,7 +32,6 @@ let dummy
       else
         let x : U16.t = read_from_buffer access_c parse32_u16 input in
         Cast.uint16_to_uint32 x
-    else 0ul
   in
   HST.pop_frame ();
   res
